# Measuring inefficiency 



## Efficient partial

$$
z'(t_e)=\frac{(1-\alpha)\left(\Lambda^o-1\right)}{\left[ 1+\left(\Lambda^o-1\right)t_e\right]^{\alpha}} 
\cdot \bar l ^{\alpha} = 0
$$

$$
t_e^0=\frac{1}{\Lambda^o-1}\cdot \left [ 
   \frac{(1-\alpha)\left(\Lambda^o-1\right)}{c}  
\right ]^\frac{1}{\alpha}\cdot \bar l
-\frac{1}{\Lambda^o-1}
$$


|                        |      |      |      |
| :--------------------: | ---- | ---- | ---- |
| $(t_e^o, l_e^o)=(0,0)$ |      |      |      |
| $(t_e^o, l_e^o)=(1,1)$ |      |      |      |
| $(t_e^o, l_e^o)=(0,0)$ |      |      |      |
|                        |      |      |      |
|                        |      |      |      |

